#import "preamble.typ": *; #show: preamble

#set heading(numbering: "1.")
#set outline.entry(fill: line(length: 100%, stroke: black.lighten(50%)))
#outline()

#v(2em)

= Dualising the LP

This is an ILP-formulation of the generalised-gasoline-problem @lucas[Figure 1.2]
$
  min thick &â€–Î²-Î±â€–_1 quad"s.t."\
  âˆ‘_(l=1)^n âˆ‘_(i=1)^m x_l Z_(i l)- âˆ‘_(i=1)^(m-1) y_i &â‰¤ Î² quad âˆ€ mâˆˆ[n]\
  âˆ‘_(l=1)^n âˆ‘_(i=1)^m x_l Z_(i l)- âˆ‘_(i=1)^m y_i &â‰¥ Î± quad âˆ€ mâˆˆ[n]\
  Z ğŸ™ &â‰¤ ğŸ™\
  ğŸ™^T Z &â‰¤ ğŸ™^T\
  Z &âˆˆ {0,1}^(n Ã— n)\
  Î±,Î² &âˆˆ â„^d
$

Before proceeding, let's introduce more notation:
- Let $ğŸ™â‰”(1,dots.c,1)^T âˆˆâ„^n$ and $ğŸ˜â‰”(0,dots.c,0)^T âˆˆ â„^n$
- Let $I$ be the $nÃ—n$ identity matrix.
- Let $L â‰” mat(1, dots.c, 0; dots.v, dots.down, dots.v; 1, dots.c, 1)$ be the $nÃ—n$ matrix with $1$ on its lower-triangle-entries (including the diagonal) and $0$ on its upper-triangle (excluding the diagonal).
- Let $y_(1:m) â‰” âˆ‘_(i=1)^m y_i$, with $y_(1:0) â‰” 0$.

We relax the ILP's integrality-constraints and rewrite it into vector-form (which later helps me dualise the LP) like this:
#pagebreak()
$
  min thick âŸ¨(ğŸ˜^T, dots.c, ğŸ˜^T, -1, 1), vâŸ© quad "s.t."&\
  mat(
    -x_1 S, -x_2 S, dots.c, -x_n S, , ğŸ˜, ğŸ™;
     //
    x_1 S, x_2 S, dots.c, x_n S, , -ğŸ™, ğŸ˜;
     //
    -I, -I, dots.c, -I, , ğŸ˜, ğŸ˜;
     //
    -ğŸ™^T, ğŸ˜^T, dots.c, ğŸ˜^T, , 0, 0;
    ğŸ˜^T, -ğŸ™^T, dots.down, dots.v, , dots.v, dots.v;
    dots.v, dots.down, dots.down, ğŸ˜^T, , 0, 0;
    ğŸ˜^T, dots.c, ğŸ˜^T, -ğŸ™^T, , 0, 0;
     //
    I, , , , , ğŸ˜, ğŸ˜;
    , I, , , , dots.v, dots.v;
    , , dots.down, , , ğŸ˜, ğŸ˜;
    , , , I, , ğŸ˜, ğŸ˜;
    augment: #(hline: (1, 2, 3, 7))
  )
  overbrace(vec(Z_(1 1), dots.v, Z_(n 1), , Z_(1 2), dots.v, Z_(n 2), , dots.v, , Z_(1 n), dots.v, Z_(n n), , Î±, Î²), â‰• v)
  &â‰¥
  mat(-y_(1:0); dots.v; -y_(1:n-1); y_(1:1); dots.v; y_(1:n); -ğŸ™; -ğŸ™; ğŸ˜; dots.v; ğŸ˜; augment: #(hline: (3, 6, 7, 8)))
$
Now that the LP is in a neat form, dualising is easy:
$
  max quad y_(1:1)â‹…a_1 +sum_(i=2)^n y_(1:i)â‹…(a_i - b_(i-1)) -âŸ¨(s_1,â€¦,s_n),ğŸ™âŸ©-âŸ¨(t_1,â€¦,t_n),ğŸ™âŸ© quad"s.t."\
  mat(
    -x_1 S^T, x_1 S^T, -I, -ğŸ™, ğŸ˜, dots.c, ğŸ˜, I, ;
    -x_2 S^T, x_2 S^T, -I, ğŸ˜, -ğŸ™, dots.down, dots.v, , I;
    dots.v, dots.v, dots.v, dots.v, dots.down, dots.down, ğŸ˜, , , dots.down;
    -x_n S^T, x_n S^T, -I, ğŸ˜, dots.c, ğŸ˜, -ğŸ™, , , , I; ;
    ğŸ˜^T, -ğŸ™^T, ğŸ˜^T, 0, dots.c, 0, 0, ğŸ˜^T, dots.c, ğŸ˜^T, ğŸ˜^T;
    ğŸ™^T, ğŸ˜^T, ğŸ˜^T, 0, dots.c, 0, 0, ğŸ˜^T, dots.c, ğŸ˜^T, ğŸ˜^T;
    augment: #(vline: (1, 2, 3, 7))
  )
  overbrace(mat(b_1; dots.v; b_n; a_1; dots.v; a_n; s_1; dots.v; s_n; t_1; dots.v; t_n; p_(1 1); dots.v; p_(n 1); p_(1 2); dots.v; dots.v; p_(1 n); dots.v; p_(n n); augment: #(hline: (3, 6, 9, 12))), â‰• w)
  = vec(ğŸ˜, dots.v, ğŸ˜, -1, 1)
  quad "and" quad wâ‰¥0
$

= Defining the instance

Fix positive integers $dâ‰¥2$ (dimension) and $kâ‰¥2$ (some parameter that, for fixed $d$, we'll send to infinity later on). Like in Lucas' thesis, define $u_i â‰” 2^k â‹… (1-2^i)$.

Recall that Lucas' $1$-dimensional instance looked like this:
$
  X &= \[underbrace(u_1\, u_1, 2^1 "times"), thick
  underbrace(u_2\, ...\, u_2, 2^2 "times"), thick
  ..., thick
  underbrace(u_(k-1)\, ...\, u_(k-1), 2^(k-1) "times"), thick
  underbrace(2^k\, ...\, 2^k, 2^(k) - 1 "times"), thick
  0\] \
  Y &= \[underbrace(u_1\, u_1, 2^1 "times"), thick
  underbrace(u_2\, ...\, u_2, 2^2 "times"), thick,
  ..., thick
  underbrace(u_(k-1)\, ...\, u_(k-1), 2^(k-1) "times"), thick
  underbrace(u^k\, ...\, u^k, 2^(k) "times")\]
$
To introduce notation (adding two lists means concatenating them, which is associative but not commutative), these $1$-dimensional instances can also be written as:
$
  X &= (âˆ‘_(i=1)^(k-1) âˆ‘_(1)^(2^i) [u_i]) + (âˆ‘_(1)^(2^k - 1) [2^k]) + [0]\
  Y &= âˆ‘_(i=1)^(k) âˆ‘_(1)^(2^i) [u_i]
$
Let $e_j = (0,â€¦,0,1,0,â€¦0)$ denote the $j$-th $d$-dimensional basis-vector.
Define a $d$-dimensional instance:
$
  X &= (âˆ‘_(i=1)^(k-1) âˆ‘_(1)^(2^i) âˆ‘_(j=2)^d [u_i e_1 + 2 e_j]) + âˆ‘_(j=2)^d ((âˆ‘_(1)^(2^k-1) [2^k e_1])+[2 e_j])\
  Y &= âˆ‘_(i=1)^(k) âˆ‘_(1)^(2^i) âˆ‘_(j=2)^d [u_i e_1 + e_j]
$

These look intimidating. @generating-code contains python-code generating these instances.

Both $X$ and $Y$ have length $2(2^k - 1)(d-1)$. The sum of the vectors in $X$ also equals the sum of the vectors in $Y$, which we won't prove here, but will _implicitly_ prove in @opt-upper-bound.

= The iterative-rounding algorithm has approximation-ratio $â‰¥d$

== The optimal value is #Green[somewhere around] $â‰¤2^k$ <opt-upper-bound>
For this, we define a permutation of the $X$ and prove it yields value $ğ’ª(2^k)$.
$
  Ï€(X)
  quadâ‰”quad
  underbrace(sum_(j=2)^d [2^k e_1,thick 2e_j], #[â‰• "First sum"])
  + underbrace(sum_(i=1)^(k-1) sum_(1)^(2^i) sum_(j=2)^d [2^k e_1,thick u_i e_1 + 2 e_j], #[â‰• "Second Sum"]),
$
This is indeed a permutation:
- The first sum is sourced from the last part of the definition of $X$.
- The second sum must therefore be a permutation of the first part of the definition of $X$ together with the remaining $âˆ‘_(1)^((d-1)â‹…(2^k-2))â‹…[2^k e_1]$. But that is true, because the second sum has exactly $(d-1)â‹…(2^(k)-2)$ summands (a "summand" being a 2-element-lists).

Remembering that $u_1=2^(k-1)$, let's take a look at the first two prefix-sums:
$
  &Ï€(X)_1 &=& 2^k e_1\
  &Ï€(X)_1 - Y_1 &=& 2^k e_1 - (2^(k-1)e_1 + e_2) &=& 2^(k-1)e_1 - e_2\
  &Ï€(X)_1 - Y_1 + Ï€(X)_2 &=& 2^(k-1)e_1 - e_2 + 2e_2 &=& 2^(k-1)e_1 + e_2\
  &Ï€(X)_1 - Y_1 + Ï€(X)_2 - Y_2 &=& 2^(k-1)e_1 + e_2 - 2^(k-1)e_1 - e_2 &=& ğŸ˜\
$
Indeed, $Ï€(X)_1 - Y_1 + Ï€(X)_2 - Y_2$. This is excellent, because it means we can always skip the first two elements when calculating the next prefix-sums.

- The proof that this applies to the first $2d$ prefix-sums is the same as the four equations above.
- The proof that this applies to the remaining prefix-sums: Having removed the initial elements, the remainder of $Ï€(X)$ and $Y$ look like this (we do an index-shift on $Y$'s $i$-sum):
  $
    "remainder of" Ï€(X) = sum_(i=1)^(k-1) sum_(1)^(2^i) sum_(j=2)^d [2^k e_1,thick u_i e_1 + 2 e_j],
    quad quad
    "remainder of" Y = âˆ‘_(i=1)^(k-1) âˆ‘_(1)^(2^(i+1)) âˆ‘_(j=2)^d [u_(i+1) e_1 + e_j]
  $
  Note that the middle sum ends at $2^i$ for $Ï€(X)$, but at $2^(i+1)$ for $Y$, but that $Ï€(X)$ sums over $2$-element-lists while $Y$ sums over $1$-element-lists. Fix any $i$. We will now look at the prefix-sums of:
  $
    XÌƒ â‰” sum_(j=2)^d [2^k e_1,thick u_i e_1 + 2 e_j],
    quad quad
    YÌƒ â‰” (âˆ‘_(j=2)^d [u_(i+1) e_1 + e_j]) + (âˆ‘_(j=2)^d [u_(i+1) e_1 + e_j])
  $
  These make up the remainder of $Ï€(X)$ and the remainder of $Y$. As we will show next, the prefix-sums of $XÌƒ$ and $YÌƒ$ sum to $0$, meaning this covers all the prefix-sums of the remainder of $Ï€(X)$ and the remainder of $Y$.

  #Green[Todo]

#Green[Todo]

== The iterative rounding algorithm achieves value #Green[somewhere around] $â‰¥ 2^k d$
_Claim_: The iterative rounding algorithm sets the first $2â‹…(2^(k-1)-1)(d-1)$ elements of $X$ in place. That is, it sets $Z_(l,l)=1$ for $1â‰¤lâ‰¤2â‹…(2^(k-1)-1)(d-1)$.

_Proof_: Assume the algorithm already set $Z_(l,l)=1$ for $1â‰¤lâ‰¤L$, for some fixed $L â‰¤ 2â‹…(2^(k-1)-1)(d-1)$. The algorithm will now try to set all $Z_(m,L+1)=1$ for $L+1â‰¤mâ‰¤n$ and will finally choose the one with smallest LP-value, breaking ties by choosing the smallest $m$. We will therefore, for all choices of $m$, calculate lower-bounds on the LP-value via the dual LP, conclude that $m=L+1$ achieves the smallest LP-value, and (being the smallest $m$) also wins the tie-break.

- #Green[Todo]



= Code

#figure(
  ```py
  import numpy as np

  d = 4
  k = 3
  xs: list[np.ndarray] = []
  ys: list[np.ndarray] = []

  for i in range(1, k):
      u = 2**k - 2 ** (k - i)
      for _ in range(2**i):
          for axis in range(1, d):
              vec = np.zeros(d, dtype=int)
              vec[0] = u
              vec[axis] = 2
              xs.append(vec)

  for axis in range(1, d):
      for _ in range(2**k - 1):
          vec = np.zeros(d, dtype=int)
          vec[0] = 2**k
          xs.append(vec)
      vec = np.zeros(d, dtype=int)
      vec[axis] = 2
      xs.append(vec)

  for i in range(1, k + 1):
      u = 2**k - 2 ** (k - i)
      for _ in range(2**i):
          for axis in range(1, d):
              vec = np.zeros(d, dtype=int)
              vec[0] = u
              vec[axis] = 1
              ys.append(vec)

  assert len(xs) == len(ys)
  assert (sum(xs) - sum(ys) == 0).all()
  ```,
  caption: [Python-Code generating the $d$-dimensional instance.],
) <generating-code>

#bibliography("bibliography.bib")

